src/tactic/refine.lean
@@ -1,11 +1,7 @@
-
 import data.dlist
-import util.control.applicative
 import meta.expr
-
-def dlist.join {α} : list (dlist α) → dlist α
- | [] := dlist.empty
- | (x :: xs) := x ++ dlist.join xs
+import tactic
+import util.control.applicative
 
 namespace expr
 
@@ -24,104 +20,70 @@ open interactive interactive.types lean.parser
      tactic.interactive (itactic)
      tactic nat applicative
 
-meta def var_names : expr → list name
- | (expr.pi n _ _ b) := n :: var_names b
- | _ := []
-
-meta def drop_binders : expr → tactic expr
- | (expr.pi n bi t b) := b.instantiate_var <$> mk_local' n bi t >>= drop_binders
- | e := pure e
-
-meta def subobject_names (struct_n : name) : tactic (list name × list name) :=
-do env ← get_env,
-   [c] ← pure $ env.constructors_of struct_n | fail "too many constructors",
-   vs  ← var_names <$> (mk_const c >>= infer_type),
-   fields ← env.structure_fields struct_n,
-   return $ fields.partition (λ fn, ↑("_" ++ fn.to_string) ∈ vs)
-
-meta def expanded_field_list' : name → tactic (dlist $ name × name) | struct_n :=
-do (so,fs) ← subobject_names struct_n,
-   -- trace so,
-   -- trace fs,
-   ts ← so.mmap (λ n, do
-     e ← mk_const (n.update_prefix struct_n) >>= infer_type >>= drop_binders,
-     expanded_field_list' $ e.get_app_fn.const_name),
-   -- trace so, trace fs,
-   -- trace $ dlist.to_list <$> ts,
-   -- trace struct_n,
-   return $ dlist.join ts ++ dlist.of_list (fs.map $ prod.mk struct_n)
 open functor function
-
-meta def expanded_field_list (struct_n : name) : tactic (list $ name × name) :=
-dlist.to_list <$> expanded_field_list' struct_n
 
 meta def qualified_field_list (struct_n : name) : tactic (list name) :=
 map (uncurry $ flip name.update_prefix) <$> expanded_field_list struct_n
 
-
-meta def mk_mvar_list : ℕ → tactic (list expr)
- | 0 := pure []
- | (succ n) := (::) <$> mk_mvar <*> mk_mvar_list n
-
 namespace interactive
 open functor
-meta def refineS (e : parse texpr) (ph : parse $ optional $ tk "with" *> ident) : tactic unit :=
-do    str ← e.get_structure_instance_info,
-      tgt ← target,
-      let struct_n : name := tgt.get_app_fn.const_name,
-      exp_fields ← expanded_field_list struct_n,
-      -- let exp_fields' := exp_fields.map prod.snd,
-      let missing_f := exp_fields.filter (λ f, (f.2 : name) ∉ str.field_names),
-      let provided  := exp_fields.filter (λ f, (f.2 : name) ∈ str.field_names),
-      vs ← mk_mvar_list missing_f.length,
-      e' ← to_expr $ pexpr.mk_structure_instance
-          { struct := some struct_n
-          , field_names  := str.field_names ++ missing_f.map prod.snd
-          , field_values := str.field_values ++ vs.map to_pexpr },
-      tactic.exact e',
-      -- trace missing_f,
-      gs ← with_enable_tags (
-        mmap₂ (λ (n : name × name) v, do
-           set_goals [v],
-           try (interactive.unfold (provided.map $ λ ⟨s,f⟩, f.update_prefix s) (loc.ns [none])),
-           -- trace n,
-           apply_auto_param
-             <|> apply_opt_param
-             <|> (set_main_tag [`_field,n.2,n.1]),
-           get_goals)
-        missing_f vs),
-      set_goals gs.join,
-      return ()
+-- meta def refineS (e : parse texpr) (ph : parse $ optional $ tk "with" *> ident) : tactic unit :=
+-- do    str ← e.get_structure_instance_info,
+--       tgt ← target,
+--       let struct_n : name := tgt.get_app_fn.const_name,
+--       exp_fields ← expanded_field_list struct_n,
+--       -- let exp_fields' := exp_fields.map prod.snd,
+--       let missing_f := exp_fields.filter (λ f, (f.2 : name) ∉ str.field_names),
+--       let provided  := exp_fields.filter (λ f, (f.2 : name) ∈ str.field_names),
+--       vs ← mk_mvar_list missing_f.length,
+--       e' ← to_expr $ pexpr.mk_structure_instance
+--           { struct := some struct_n
+--           , field_names  := str.field_names ++ missing_f.map prod.snd
+--           , field_values := str.field_values ++ vs.map to_pexpr },
+--       tactic.exact e',
+--       -- trace missing_f,
+--       gs ← with_enable_tags (
+--         mmap₂ (λ (n : name × name) v, do
+--            set_goals [v],
+--            try (interactive.unfold (provided.map $ λ ⟨s,f⟩, f.update_prefix s) (loc.ns [none])),
+--            -- trace n,
+--            apply_auto_param
+--              <|> apply_opt_param
+--              <|> (set_main_tag [`_field,n.2,n.1]),
+--            get_goals)
+--         missing_f vs),
+--       set_goals gs.join,
+--       return ()
 
-meta def collect_tagged_goals (pre : name) : tactic (list expr) :=
-do gs ← get_goals,
-   gs.mfoldr (λ g r, do
-      pre' :: t ← get_tag g,
-      if t = [pre] ∧ pre' = pre'.get_prefix <.> "_field"
-         then return (g::r)
-         else return r)
-      []
+-- meta def collect_tagged_goals (pre : name) : tactic (list expr) :=
+-- do gs ← get_goals,
+--    gs.mfoldr (λ g r, do
+--       pre' :: t ← get_tag g,
+--       if t = [pre] ∧ pre' = pre'.get_prefix <.> "_field"
+--          then return (g::r)
+--          else return r)
+--       []
 
--- meta def match_field_tag
+-- -- meta def match_field_tag
 
-meta def field (tag : parse ident) (tac : itactic) : tactic unit :=
-do ts ← collect_tagged_goals tag,
-   match ts with
-    | [] := fail format!"no field goal with tag {tag}"
-    | [g] := do
-      gs ← get_goals,
-      set_goals $ g :: gs.filter (≠ g),
-      solve1 tac
-    | _ := fail format!"multiple goals have tag {tag}"
-   end
+-- meta def field (tag : parse ident) (tac : itactic) : tactic unit :=
+-- do ts ← collect_tagged_goals tag,
+--    match ts with
+--     | [] := fail format!"no field goal with tag {tag}"
+--     | [g] := do
+--       gs ← get_goals,
+--       set_goals $ g :: gs.filter (≠ g),
+--       solve1 tac
+--     | _ := fail format!"multiple goals have tag {tag}"
+--    end
 
-meta def get_current_field (t : name) : tactic name :=
-do [_,field,str] ← get_main_tag,
-   -- trace format!"{field} - {str}",
-   expr.const_name <$> resolve_name (field.update_prefix str)
+-- meta def get_current_field : tactic name :=
+-- do [_,field,str] ← get_main_tag,
+--    -- trace format!"{field} - {str}",
+--    expr.const_name <$> resolve_name (field.update_prefix str)
 
--- meta def current_field (t : name) (c : name := `current) : tactic unit :=
--- () <$ (get_current_field t >>= mk_const >>= pose c none)
+-- -- meta def current_field (t : name) (c : name := `current) : tactic unit :=
+-- -- () <$ (get_current_field t >>= mk_const >>= pose c none)
 
 end interactive
 
